theories/prob_eff_lang/probblaze/examples/DH_KE/dhke_channel.v
@@ -971,7 +971,7 @@ Section handlee_verification.
                                             BREL v1 ((λ: "m", do: c1 (Send "m")), (λ: "m", do: c1 (Recv "m")))%V ≤
                                                  v2 ((λ: "m", do: c2 (Send "m")), (λ: "m", do: c2 (Recv "m")))%V 
                                                  <| (iLblSig_to_iLblThy ac) ++ (iLblSig_to_iLblThy L) |> {{ (λ w1 w2, 𝟙%T w1 w2) }} }} -∗
-    BREL F_AUTH f1 ≤ F_AUTH f2 <| ⊥ |> {{ λ v1 v2, 
+    BREL F_AUTH_legacy f1 ≤ F_AUTH_legacy f2 <| ⊥ |> {{ λ v1 v2, 
                                                                 (∀ᵣ θₗ, (((⊤ × (𝟙 + 𝟙)) -{ θₗ }-> 𝟙) × ((𝟙 + 𝟙) -{ θₗ }-> Option ⊤)) -{ sem_row_union θₗ L }-∘ 𝟙)%T v1 v2 }}.
   Proof with (repeat foldkont) using G. 
     iIntros "Hfraca Hfracb Hff". 
@@ -981,7 +981,7 @@ Section handlee_verification.
     iApply (brel_mono OS _ _ ⊥ [] with "[][$Hff]"); [iApply to_iThy_le_bot|simpl].
     clear f1 f2.
     iIntros (f1 f2) "Hff". 
-    unfold F_AUTH.
+    unfold F_AUTH_legacy.
     brel_pures'. iModIntro.
     iIntros (sendrecv). iIntros (sr1 sr2) "(%send1&%send2&%recv1&%recv2&->&->&(#Hsend&#Hrecv))".
     (* iIntros (lc dsend1 dsend2) "#Hsend". 
@@ -1277,7 +1277,7 @@ Section handlee_verification.
 
 
   Lemma F_AUTH_DH_KE_FAUTH_C_DH_real :
-    ⊢ sem_val_typed (λ: "f", F_AUTH (DH_KE "f"))%V (λ: "f", F_AUTH (C DH_real "f"))%V  
+    ⊢ sem_val_typed (λ: "f", F_AUTH_legacy (DH_KE "f"))%V (λ: "f", F_AUTH_legacy (C DH_real "f"))%V  
                          (∀ᵣ θ__L, (∀ᵣ θₕ, ((sem_ty_sum 𝟙 𝟙) -{ θₕ }-> (Option 𝔾)) -{ sem_row_union θₕ θ__L }-∘ 𝟙)%T ⊸ ((∀ᵣ θₗ, (((⊤ × (𝟙 + 𝟙)) -{ θₗ }-> 𝟙) × ((𝟙 + 𝟙) -{ θₗ }-> Option ⊤)) -{ sem_row_union θₗ θ__L }-∘ 𝟙)))%T.
   Proof using G channel1 channel2 inG0 inG1 inG2. (* TODO: remove channel1 channel2 from context *)
     iModIntro. iIntros (L).
@@ -1301,7 +1301,7 @@ Section handlee_verification.
   (* Verification of F_AUTH[C[DH_real]] ≤ F_AUTH[DH_KE] *)
   (*------------------------------------------------------------*)
   Lemma F_AUTH_C_DH_real_FAUTH_DH_KE :
-     ⊢ sem_val_typed (λ: "f", F_AUTH (C DH_real "f"))%V (λ: "f", F_AUTH (DH_KE "f"))%V  
+     ⊢ sem_val_typed (λ: "f", F_AUTH_legacy (C DH_real "f"))%V (λ: "f", F_AUTH_legacy (DH_KE "f"))%V  
                          (∀ᵣ θ__L, (∀ᵣ θₕ, ((sem_ty_sum 𝟙 𝟙) -{ θₕ }-> (Option 𝔾)) -{ sem_row_union θₕ θ__L }-∘ 𝟙)%T ⊸ ((∀ᵣ θₗ, (((⊤ × (𝟙 + 𝟙)) -{ θₗ }-> 𝟙) × ((𝟙 + 𝟙) -{ θₗ }-> Option ⊤)) -{ sem_row_union θₗ θ__L }-∘ 𝟙)))%T.
   Proof using G channel1 channel2 inG0 inG1 inG2.
     iModIntro. iIntros (L).
@@ -1970,7 +1970,7 @@ Section handlee_verification.
   (* Verification of F_AUTH[DH_SIM[F_KE]] ≤ F_AUTH[C[DH_rand]] *)
   (*------------------------------------------------------------*)
   Lemma F_AUTH_DH_SIM_F_KE_FAUTH_C_DH_rand :
-     ⊢ sem_val_typed (λ: "f", F_AUTH (DH_SIM (F_KE "f")))%V (λ: "f", F_AUTH (C DH_rand "f"))%V  
+     ⊢ sem_val_typed (λ: "f", F_AUTH_legacy (DH_SIM (F_KE "f")))%V (λ: "f", F_AUTH_legacy (C DH_rand "f"))%V  
                          (∀ᵣ θ__L, (∀ᵣ θₕ, ((sem_ty_sum 𝟙 𝟙) -{ θₕ }-> (Option 𝔾)) -{ sem_row_union θₕ θ__L }-∘ 𝟙)%T ⊸ ((∀ᵣ θₗ, (((⊤ × (𝟙 + 𝟙)) -{ θₗ }-> 𝟙) × ((𝟙 + 𝟙) -{ θₗ }-> Option ⊤)) -{ sem_row_union θₗ θ__L }-∘ 𝟙)))%T.
   Proof using G channel1 channel2 inG0 inG1 inG2.
     iModIntro. iIntros (L).
@@ -1994,7 +1994,7 @@ Section handlee_verification.
   (* Verification of F_AUTH[C[DH_rand]] ≤ F_AUTH[DH_SIM[F_KE]] *)
   (*------------------------------------------------------------*)
   Lemma F_AUTH_C_DH_rand_FAUTH_DH_SIM_F_KE :
-    ⊢ sem_val_typed (λ: "f", F_AUTH (C DH_rand "f"))%V (λ: "f", F_AUTH (DH_SIM (F_KE "f")))%V  
+    ⊢ sem_val_typed (λ: "f", F_AUTH_legacy (C DH_rand "f"))%V (λ: "f", F_AUTH_legacy (DH_SIM (F_KE "f")))%V  
         (∀ᵣ θ__L, (∀ᵣ θₕ, ((sem_ty_sum 𝟙 𝟙) -{ θₕ }-> (Option 𝔾)) -{ sem_row_union θₕ θ__L }-∘ 𝟙)%T ⊸ ((∀ᵣ θₗ, (((⊤ × (𝟙 + 𝟙)) -{ θₗ }-> 𝟙) × ((𝟙 + 𝟙) -{ θₗ }-> Option ⊤)) -{ sem_row_union θₗ θ__L }-∘ 𝟙)))%T.
   Proof using channel1 channel2 G inG0 inG1 inG2.
     iModIntro. iIntros (L).
@@ -2018,7 +2018,7 @@ Section handlee_verification.
   (* Rewriting to match top-level statements *)
   (*------------------------------------------------------------*)
   Lemma DHSIM_RED : 
-    ⊢ sem_typed [] (λ: "f", F_AUTH (DH_SIM (F_KE "f")))%V ((λ: "DH" "f", F_AUTH (C "DH" "f"))%V DH_rand) ⊥ (∀ᵣ θ__L, (∀ᵣ θₕ, ((sem_ty_sum 𝟙 𝟙) -{ θₕ }-> (Option 𝔾)) -{ sem_row_union θₕ θ__L }-∘ 𝟙)%T ⊸ ((∀ᵣ θₗ, (((⊤ × (𝟙 + 𝟙)) -{ θₗ }-> 𝟙) × ((𝟙 + 𝟙) -{ θₗ }-> Option ⊤)) -{ sem_row_union θₗ θ__L }-∘ 𝟙)))%T [].
+    ⊢ sem_typed [] (λ: "f", F_AUTH_legacy (DH_SIM (F_KE "f")))%V ((λ: "DH" "f", F_AUTH_legacy (C "DH" "f"))%V DH_rand) ⊥ (∀ᵣ θ__L, (∀ᵣ θₕ, ((sem_ty_sum 𝟙 𝟙) -{ θₕ }-> (Option 𝔾)) -{ sem_row_union θₕ θ__L }-∘ 𝟙)%T ⊸ ((∀ᵣ θₗ, (((⊤ × (𝟙 + 𝟙)) -{ θₗ }-> 𝟙) × ((𝟙 + 𝟙) -{ θₗ }-> Option ⊤)) -{ sem_row_union θₗ θ__L }-∘ 𝟙)))%T [].
   Proof using G channel1 channel2 inG0 inG1 inG2.
     iIntros (vs) "!# _". simpl.
     brel_pures'.
@@ -2028,7 +2028,7 @@ Section handlee_verification.
   Qed. 
   
   Lemma RED_DHSIM :
-    ⊢ sem_typed [] ((λ: "DH" "f", F_AUTH (C "DH" "f"))%V DH_rand) (λ: "f", F_AUTH (DH_SIM (F_KE "f")))%V ⊥ (∀ᵣ θ__L, (∀ᵣ θₕ, ((sem_ty_sum 𝟙 𝟙) -{ θₕ }-> (Option 𝔾)) -{ sem_row_union θₕ θ__L }-∘ 𝟙)%T ⊸ ((∀ᵣ θₗ, (((⊤ × (𝟙 + 𝟙)) -{ θₗ }-> 𝟙) × ((𝟙 + 𝟙) -{ θₗ }-> Option ⊤)) -{ sem_row_union θₗ θ__L }-∘ 𝟙)))%T [].
+    ⊢ sem_typed [] ((λ: "DH" "f", F_AUTH_legacy (C "DH" "f"))%V DH_rand) (λ: "f", F_AUTH_legacy (DH_SIM (F_KE "f")))%V ⊥ (∀ᵣ θ__L, (∀ᵣ θₕ, ((sem_ty_sum 𝟙 𝟙) -{ θₕ }-> (Option 𝔾)) -{ sem_row_union θₕ θ__L }-∘ 𝟙)%T ⊸ ((∀ᵣ θₗ, (((⊤ × (𝟙 + 𝟙)) -{ θₗ }-> 𝟙) × ((𝟙 + 𝟙) -{ θₗ }-> Option ⊤)) -{ sem_row_union θₗ θ__L }-∘ 𝟙)))%T [].
   Proof using G channel1 channel2 inG0 inG1 inG2.
     iIntros (vs) "!# _". simpl.
     brel_pures'.
@@ -2038,7 +2038,7 @@ Section handlee_verification.
   Qed.  
   
   Lemma DHKE_RED :
-    ⊢ sem_typed [] (λ: "f", F_AUTH (DH_KE "f"))%V ((λ: "DH" "f", F_AUTH (C "DH" "f"))%V DH_real) ⊥
+    ⊢ sem_typed [] (λ: "f", F_AUTH_legacy (DH_KE "f"))%V ((λ: "DH" "f", F_AUTH_legacy (C "DH" "f"))%V DH_real) ⊥
                          (∀ᵣ θ__L, (∀ᵣ θₕ, ((sem_ty_sum 𝟙 𝟙) -{ θₕ }-> (Option 𝔾)) -{ sem_row_union θₕ θ__L }-∘ 𝟙)%T ⊸ ((∀ᵣ θₗ, (((⊤ × (𝟙 + 𝟙)) -{ θₗ }-> 𝟙) × ((𝟙 + 𝟙) -{ θₗ }-> Option ⊤)) -{ sem_row_union θₗ θ__L }-∘ 𝟙)))%T [].
   Proof using G channel1 channel2 inG0 inG1 inG2.
     iIntros (vs) "!# _". simpl.
@@ -2049,7 +2049,7 @@ Section handlee_verification.
   Qed.  
   
   Lemma RED_DHKE :
-    ⊢ sem_typed [] ((λ: "DH" "f", F_AUTH (C "DH" "f"))%V DH_real) (λ: "f", F_AUTH (DH_KE "f"))%V ⊥
+    ⊢ sem_typed [] ((λ: "DH" "f", F_AUTH_legacy (C "DH" "f"))%V DH_real) (λ: "f", F_AUTH_legacy (DH_KE "f"))%V ⊥
         (∀ᵣ θ__L, (∀ᵣ θₕ, ((sem_ty_sum 𝟙 𝟙) -{ θₕ }-> (Option 𝔾)) -{ sem_row_union θₕ θ__L }-∘ 𝟙)%T ⊸ ((∀ᵣ θₗ, (((⊤ × (𝟙 + 𝟙)) -{ θₗ }-> 𝟙) × ((𝟙 + 𝟙) -{ θₗ }-> Option ⊤)) -{ sem_row_union θₗ θ__L }-∘ 𝟙)))%T [].
   Proof using G channel1 channel2 inG0 inG1 inG2.
     iIntros (vs) "!# _". simpl.
